Added silent variables in target lambda calculus

doc/formalization/Catala.LambdaCalculus.fst
@@ -10,7 +10,11 @@ type ty =
   | TList: elts:ty -> ty
   | TOption: a: ty -> ty
 
-type var = int
+type var_name = nat
+
+type var =
+  | Named of var_name
+  | Silent
 
 type err =
   | EmptyError : err
@@ -23,7 +27,7 @@ type lit =
   | LUnit : lit
 
 type exp =
-  | EVar : v: var -> exp
+  | EVar : v: var_name -> exp
   | EApp : fn: exp -> arg: exp -> tau_arg: ty -> exp
   | EAbs : v: var -> vty: ty -> body: exp -> exp
   | ELit : l: lit -> exp
@@ -56,10 +60,10 @@ and is_value_list (es: list exp) : Tot bool =
   | hd::tl -> is_value hd && is_value_list tl
 
 
-let rec subst (x: var) (e_x e: exp) : Tot exp (decreases e) =
+let rec subst (x: var_name) (e_x e: exp) : Tot exp (decreases e) =
   match e with
   | EVar x' -> if x = x' then e_x else e
-  | EAbs x' t e1 -> EAbs x' t (if x = x' then e1 else (subst x e_x e1))
+  | EAbs x' t e1 -> EAbs x' t (if Named x = x' then e1 else (subst x e_x e1))
   | EApp e1 e2 tau_arg -> EApp (subst x e_x e1) (subst x e_x e2) tau_arg
   | ELit l -> ELit l
   | EIf e1 e2 e3 -> EIf (subst x e_x e1) (subst x e_x e2) (subst x e_x e3)
@@ -72,7 +76,7 @@ let rec subst (x: var) (e_x e: exp) : Tot exp (decreases e) =
     ECatchEmptyError (subst x e_x to_try) (subst x e_x catch_with)
   | EFoldLeft f init tau_init l tau_elt ->
     EFoldLeft (subst x e_x f) (subst x e_x init) tau_init (subst x e_x l) tau_elt
-and subst_list (x: var) (e_x: exp) (subs: list exp) : Tot (list exp) (decreases subs) =
+and subst_list (x: var_name) (e_x: exp) (subs: list exp) : Tot (list exp) (decreases subs) =
   match subs with
   | [] -> []
   | hd :: tl -> (subst x e_x hd) :: (subst_list x e_x tl)
@@ -92,7 +96,8 @@ let rec step_app (e: exp) (e1: exp{e1 << e}) (e2: exp{e2 << e}) (tau_arg: ty{tau
         | ELit (LError err) -> Some (ELit (LError err))
         | _ -> begin
           match e1 with
-          | EAbs x t e' -> Some (subst x e2 e') (* D-Beta *)
+          | EAbs (Named x) t e' -> Some (subst x e2 e') (* D-Beta *)
+          | EAbs Silent t e' -> Some e' (* D-Beta *)
           | _ -> None
         end
       else
@@ -227,13 +232,14 @@ and step (e: exp) : Tot (option exp) (decreases %[ e; 6 ]) =
 
 (**** Typing helpers *)
 
-type env = FunctionalExtensionality.restricted_t var (fun _ -> option ty)
+type env = FunctionalExtensionality.restricted_t var_name (fun _ -> option ty)
 
 val empty:env
-let empty = FunctionalExtensionality.on_dom var (fun _ -> None)
+let empty = FunctionalExtensionality.on_dom var_name (fun _ -> None)
 
-val extend: env -> var -> ty -> Tot env
-let extend g x t = FunctionalExtensionality.on_dom var (fun x' -> if x = x' then Some t else g x')
+val extend: env -> var_name -> ty -> Tot env
+let extend g x t = FunctionalExtensionality.on_dom var_name
+  (fun x' -> if x = x' then Some t else g x')
 
 (**** Typing judgment *)
 
@@ -242,7 +248,8 @@ let rec typing (g: env) (e: exp) (tau: ty) : Tot bool (decreases (e)) =
   | EVar x -> g x = Some tau
   | EAbs x t e1 ->
     (match tau with
-      | TArrow tau_in tau_out -> t = tau_in && typing (extend g x t) e1 tau_out
+      | TArrow tau_in tau_out -> t = tau_in &&
+        typing (match x with Named x -> extend g x t | Silent -> g) e1 tau_out
       | _ -> false)
   | EApp e1 e2 tau_arg -> typing g e1 (TArrow tau_arg tau) && typing g e2 tau_arg
   | ELit LTrue -> tau = TBool
@@ -348,15 +355,19 @@ let lemma_size_fold_step (f init hd: exp) (tl: list exp) (tau_init tau_elt: ty) 
   )
 #pop-options
 
+#push-options "--fuel 1 --ifuel 0 --z3rlimit 30"
 let lemma_size_fold_f (f init l: exp) (tau_init tau_elt: ty)
     : Lemma (size_for_progress (EFoldLeft f init tau_init l tau_elt) > size_for_progress f)
   =
   ()
+#pop-options
 
+#push-options "--fuel 1 --ifuel 0 --z3rlimit 30"
 let lemma_size_fold_init (f init l: exp) (tau_init tau_elt: ty)
     : Lemma (size_for_progress (EFoldLeft f init tau_init l tau_elt) > size_for_progress init)
   =
   ()
+#pop-options
 
 #push-options "--fuel 1 --ifuel 0 --z3rlimit 30"
 let lemma_size_fold_l (f init l: exp) (tau_init tau_elt: ty)
@@ -365,7 +376,7 @@ let lemma_size_fold_l (f init l: exp) (tau_init tau_elt: ty)
   ()
 #pop-options
 
-#push-options "--fuel 3 --ifuel 1 --z3rlimit 50"
+#push-options "--fuel 3 --ifuel 2 --z3rlimit 50"
 let rec progress (e: exp) (tau: ty)
     : Lemma (requires (typing empty e tau))
       (ensures (is_value e \/ (Some? (step e))))
@@ -449,30 +460,31 @@ and progress_list
 
 (**** Preservation helpers *)
 
-let rec appears_free_in (x: var) (e: exp) : Tot bool =
+let rec appears_free_in (x: var_name) (e: exp) : Tot bool =
   match e with
   | EVar y -> x = y
   | EApp e1 e2 _ | ECatchEmptyError e1 e2 -> appears_free_in x e1 || appears_free_in x e2
-  | EAbs y _ e1 -> x <> y && appears_free_in x e1
+  | EAbs y _ e1 -> Named x <> y && appears_free_in x e1
   | EIf e1 e2 e3 | EMatchOption e1 _ e2 e3 | EFoldLeft e1 e2 _ e3 _ ->
     appears_free_in x e1 || appears_free_in x e2 || appears_free_in x e3
   | ESome e1 -> appears_free_in x e1
   | EList e1 -> appears_free_in_list x e1
   | ENone | ELit _ -> false
-and appears_free_in_list (x: var) (subs: list exp) : Tot bool =
+and appears_free_in_list (x: var_name) (subs: list exp) : Tot bool =
   match subs with
   | [] -> false
   | hd :: tl -> appears_free_in x hd || appears_free_in_list x tl
 
 #push-options "--fuel 2 --ifuel 1"
-let rec free_in_context (x: var) (e: exp) (g: env) (tau: ty)
+let rec free_in_context (x: var_name) (e: exp) (g: env) (tau: ty)
     : Lemma (requires (typing g e tau))
       (ensures (appears_free_in x e ==> Some? (g x)))
       (decreases e) =
   match e with
   | EVar _ | ELit _ -> ()
   | EAbs y t e1 ->
-    (match tau with | TArrow _ tau_out -> free_in_context x e1 (extend g y t) tau_out)
+    (match tau with | TArrow _ tau_out ->
+      free_in_context x e1 (match y with Named y -> extend g y t | Silent -> g) tau_out)
   | EApp e1 e2 tau_arg ->
     free_in_context x e1 g (TArrow tau_arg tau);
     free_in_context x e2 g tau_arg
@@ -502,7 +514,7 @@ let rec free_in_context (x: var) (e: exp) (g: env) (tau: ty)
     free_in_context x init g tau_init;
     free_in_context x l g (TList tau_elt);
     free_in_context x f g (TArrow tau_init (TArrow tau_elt tau_init))
-and free_in_context_list (x: var) (subs: list exp) (g: env) (tau: ty)
+and free_in_context_list (x: var_name) (subs: list exp) (g: env) (tau: ty)
     : Lemma (requires (typing_list g subs tau))
       (ensures (appears_free_in_list x subs ==> Some? (g x)))
       (decreases subs) =
@@ -513,7 +525,7 @@ and free_in_context_list (x: var) (subs: list exp) (g: env) (tau: ty)
     free_in_context_list x tl g tau
 #pop-options
 
-let typable_empty_closed (x: var) (e: exp) (tau: ty)
+let typable_empty_closed (x: var_name) (e: exp) (tau: ty)
     : Lemma (requires (typing empty e tau))
       (ensures (not (appears_free_in x e)))
       [SMTPat (appears_free_in x e); SMTPat (typing empty e tau)] =
@@ -521,12 +533,12 @@ let typable_empty_closed (x: var) (e: exp) (tau: ty)
 
 (**** Context invariance *)
 
-type equal (g1: env) (g2: env) = forall (x: var). g1 x = g2 x
+type equal (g1: env) (g2: env) = forall (x: var_name). g1 x = g2 x
 
-type equalE (e: exp) (g1: env) (g2: env) = forall (x: var). appears_free_in x e ==> g1 x = g2 x
+type equalE (e: exp) (g1: env) (g2: env) = forall (x: var_name). appears_free_in x e ==> g1 x = g2 x
 
 type equalE_list (subs: list exp) (g1: env) (g2: env) =
-  forall (x: var). appears_free_in_list x subs ==> g1 x = g2 x
+  forall (x: var_name). appears_free_in_list x subs ==> g1 x = g2 x
 
 #push-options "--fuel 2 --ifuel 1"
 let rec context_invariance (e: exp) (g g': env) (tau: ty)
@@ -536,7 +548,11 @@ let rec context_invariance (e: exp) (g g': env) (tau: ty)
   match e with
   | EAbs x t e1 ->
     (match tau with
-      | TArrow _ tau_out -> context_invariance e1 (extend g x t) (extend g' x t) tau_out
+      | TArrow _ tau_out -> begin
+        match x with
+        | Named x -> context_invariance e1 (extend g x t) (extend g' x t) tau_out
+        | Silent -> context_invariance e1 g g' tau_out
+      end
       | _ -> ())
   | EApp e1 e2 tau_arg ->
     context_invariance e1 g g' (TArrow tau_arg tau);
@@ -586,7 +602,7 @@ let typing_extensional (g g': env) (e: exp) (tau: ty)
 (**** Substitution preservation *)
 
 #push-options "--fuel 1 --ifuel 1 --z3rlimit 10"
-let rec substitution_preserves_typing (x: var) (tau_x: ty) (e v: exp) (g: env) (tau: ty)
+let rec substitution_preserves_typing (x: var_name) (tau_x: ty) (e v: exp) (g: env) (tau: ty)
     : Lemma (requires (typing empty v tau_x /\ typing (extend g x tau_x) e tau))
       (ensures (typing g (subst x v e) tau))
       (decreases %[ e ]) =
@@ -605,15 +621,19 @@ let rec substitution_preserves_typing (x: var) (tau_x: ty) (e v: exp) (g: env) (
     (match tau with
       | TArrow tau_in tau_out ->
         if tau_in = t_y
-        then
-          let gxy = extend gx y t_y in
-          let gy = extend g y t_y in
-          if x = y
-          then typing_extensional gxy gy e1 tau_out
-          else
-            let gyx = extend gy x tau_x in
-            typing_extensional gxy gyx e1 tau_out;
-            substitution_preserves_typing x tau_x e1 v gy tau_out
+        then begin
+          match y with
+          | Named y ->
+            let gxy = extend gx y t_y in
+            let gy = extend g y t_y in
+            if x = y
+            then typing_extensional gxy gy e1 tau_out
+            else
+              let gyx = extend gy x tau_x in
+              typing_extensional gxy gyx e1 tau_out;
+              substitution_preserves_typing x tau_x e1 v gy tau_out
+          | Silent -> substitution_preserves_typing x tau_x e1 v g tau_out
+        end
       | _ -> ())
   | ESome s ->
     (match tau with
@@ -636,7 +656,7 @@ let rec substitution_preserves_typing (x: var) (tau_x: ty) (e v: exp) (g: env) (
     substitution_preserves_typing x tau_x init v g tau_init;
     substitution_preserves_typing x tau_x l v g (TList tau_elt)
 and substitution_preserves_typing_list
-      (x: var)
+      (x: var_name)
       (tau_x: ty)
       (exceptions: list exp)
       (v: exp)
@@ -672,7 +692,8 @@ let rec preservation (e: exp) (tau: ty)
         if is_value e2
         then
           match e1 with
-          | EAbs x _ ebody -> substitution_preserves_typing x tau_arg ebody e2 empty tau
+          | EAbs (Named x) _ ebody -> substitution_preserves_typing x tau_arg ebody e2 empty tau
+          | EAbs Silent _ ebody -> ()
           | _ -> ()
         else preservation e2 tau_arg
     else preservation e1 (TArrow tau_arg tau)
